code/hash/Hacl.Impl.SHA2.Core.fsti
@@ -10,7 +10,7 @@ open Lib.IntVector
 open Spec.Hash.Definitions
 open Hacl.Hash.Definitions
 
-val sha256: hash:lbuffer uint8 32ul -> len:size_t -> b:buffer uint8{length b == v len} ->
+val sha256: hash:lbuffer uint8 32ul -> len:size_t -> b:lbuffer uint8 len ->
     Stack unit
     (requires (fun h0 -> live h0 b /\ live h0 hash /\ disjoint hash b))
     (ensures (fun h0 _ h1 -> modifies (loc hash) h0 h1))
@@ -20,10 +20,10 @@ val sha256_4: r0:lbuffer uint8 32ul ->
               r2:lbuffer uint8 32ul ->
               r3:lbuffer uint8 32ul ->
               len:size_t ->
-              b0:buffer uint8{length b0 == v len} ->
-              b1:buffer uint8{length b1 == v len} ->
-              b2:buffer uint8{length b2 == v len} ->
-              b3:buffer uint8{length b3 == v len} ->
+              b0:lbuffer uint8 len ->
+              b1:lbuffer uint8 len ->
+              b2:lbuffer uint8 len ->
+              b3:lbuffer uint8 len ->
     Stack unit
     (requires (fun h0 -> live h0 b0 /\ live h0 b1 /\ live h0 b2 /\ live h0 b3 /\ 
                        live h0 r0 /\ live h0 r1 /\ live h0 r2 /\ live h0 r3))
